Cslib/Computability/Automata/NFAToDFA.lean
@@ -13,7 +13,7 @@ namespace Cslib
 
 namespace NFA
 
-variable {State : Type _} {Symbol : Type _}
+variable {State : Type*} {Symbol : Type*}
 
 section SubsetConstruction
 
