Cslib/Computability/Languages/RegularLanguage.lean
@@ -18,9 +18,10 @@ open scoped Computability
 
 namespace Language
 
-variable {Symbol : Type _} [Finite Symbol]
+variable {Symbol : Type*} [Finite Symbol]
 
-theorem regular_iff_cslib_dfa {l : Language Symbol} :
+/-- A characterization of Language.IsRegular using Cslib.DFA -/
+theorem IsRegular.iff_cslib_dfa {l : Language Symbol} :
     l.IsRegular ↔ ∃ State : Type, ∃ dfa : Cslib.DFA State Symbol, dfa.language = l := by
   constructor
   · rintro ⟨State, h_State, dfa, rfl⟩
@@ -41,9 +42,10 @@ theorem regular_iff_cslib_dfa {l : Language Symbol} :
     use State, (Fintype.ofFinite State), dfa'
     rfl
 
-theorem regular_iff_cslib_nfa {l : Language Symbol} :
+/-- A characterization of Language.IsRegular using Cslib.NFA -/
+theorem IsRegular.iff_cslib_nfa {l : Language Symbol} :
     l.IsRegular ↔ ∃ State : Type, ∃ nfa : Cslib.NFA State Symbol, nfa.language = l := by
-  rw [regular_iff_cslib_dfa] ; constructor
+  rw [IsRegular.iff_cslib_dfa] ; constructor
   · rintro ⟨State, dfa, rfl⟩
     use State, dfa.toNFA
     exact Cslib.DFA.toNFA_language_eq
@@ -51,76 +53,76 @@ theorem regular_iff_cslib_nfa {l : Language Symbol} :
     use (Set State), nfa.toDFA
     exact Cslib.NFA.toDFA_language_eq
 
+-- From this point onward we will use only automata from Cslib in the proofs.
 open Cslib
 
 @[simp]
-theorem regular_compl {l : Language Symbol} (h : l.IsRegular) : (lᶜ).IsRegular := by
-  rw [regular_iff_cslib_dfa] at h ⊢
+theorem IsRegular.compl {l : Language Symbol} (h : l.IsRegular) : (lᶜ).IsRegular := by
+  rw [IsRegular.iff_cslib_dfa] at h ⊢
   obtain ⟨State, dfa, rfl⟩ := h
   use State, dfa.compl
   simp
 
 @[simp]
-theorem regular_zero : (0 : Language Symbol).IsRegular := by
-  rw [regular_iff_cslib_dfa]
+theorem IsRegular.zero : (0 : Language Symbol).IsRegular := by
+  rw [IsRegular.iff_cslib_dfa]
   use Unit, DFA.zero
   simp
 
 @[simp]
-theorem regular_one : (1 : Language Symbol).IsRegular := by
-  rw [regular_iff_cslib_dfa]
+theorem IsRegular.one : (1 : Language Symbol).IsRegular := by
+  rw [IsRegular.iff_cslib_dfa]
   use Fin 2, DFA.one
   simp
 
 @[simp]
-theorem regular_top : (⊤ : Language Symbol).IsRegular := by
-  have : (⊥ᶜ : Language Symbol).IsRegular := regular_compl <| regular_zero (Symbol := Symbol)
+theorem IsRegular.top : (⊤ : Language Symbol).IsRegular := by
+  have : (⊥ᶜ : Language Symbol).IsRegular := IsRegular.compl <| IsRegular.zero (Symbol := Symbol)
   rwa [← compl_bot]
 
 @[simp]
-theorem regular_inf {l1 l2 : Language Symbol}
+theorem IsRegular.inf {l1 l2 : Language Symbol}
     (h1 : l1.IsRegular) (h2 : l2.IsRegular) : (l1 ⊓ l2).IsRegular := by
-  rw [regular_iff_cslib_dfa] at h1 h2 ⊢
+  rw [IsRegular.iff_cslib_dfa] at h1 h2 ⊢
   obtain ⟨State1, dfa1, rfl⟩ := h1
   obtain ⟨State2, dfa2, rfl⟩ := h2
   use (State1 × State2), (dfa1.inf dfa2)
   simp
 
 @[simp]
-theorem regular_add {l1 l2 : Language Symbol}
+theorem IsRegular.add {l1 l2 : Language Symbol}
     (h1 : l1.IsRegular) (h2 : l2.IsRegular) : (l1 + l2).IsRegular := by
-  rw [regular_iff_cslib_dfa] at h1 h2 ⊢
+  rw [IsRegular.iff_cslib_dfa] at h1 h2 ⊢
   obtain ⟨State1, dfa1, rfl⟩ := h1
   obtain ⟨State2, dfa2, rfl⟩ := h2
   use (State1 × State2), (dfa1.add dfa2)
   simp
 
 @[simp]
-theorem regular_iInf {I : Type _} [Finite I] {s : Set I} {l : I → Language Symbol}
+theorem IsRegular.iInf {I : Type*} [Finite I] {s : Set I} {l : I → Language Symbol}
     (h : ∀ i ∈ s, (l i).IsRegular) : (⨅ i ∈ s, l i).IsRegular := by
   generalize h_n : s.ncard = n
   induction n generalizing s
   case zero =>
     obtain ⟨rfl⟩ := (ncard_eq_zero (s := s)).mp h_n
-    simp only [mem_empty_iff_false, not_false_eq_true, iInf_neg, iInf_top]
-    exact regular_top
+    simp
   case succ n h_ind =>
     obtain ⟨i, t, h_i, rfl, rfl⟩ := (ncard_eq_succ (s := s)).mp h_n
-    rw [biInf_insert]
-    apply regular_inf <;> grind
+    rw [iInf_insert]
+    grind [IsRegular.inf]
 
 @[simp]
-theorem regular_iSup {I : Type _} [Finite I] {s : Set I} {l : I → Language Symbol}
+theorem IsRegular.iSup {I : Type*} [Finite I] {s : Set I} {l : I → Language Symbol}
     (h : ∀ i ∈ s, (l i).IsRegular) : (⨆ i ∈ s, l i).IsRegular := by
   generalize h_n : s.ncard = n
   induction n generalizing s
   case zero =>
     obtain ⟨rfl⟩ := (ncard_eq_zero (s := s)).mp h_n
     simp only [mem_empty_iff_false, not_false_eq_true, iSup_neg, iSup_bot]
-    exact regular_zero
+    exact IsRegular.zero
   case succ n h_ind =>
     obtain ⟨i, t, h_i, rfl, rfl⟩ := (ncard_eq_succ (s := s)).mp h_n
-    rw [biSup_insert]
-    apply regular_add <;> grind
+    rw [iSup_insert]
+    apply IsRegular.add <;> grind
 
 end Language
